src/versions/standard/Int63/Int63Axioms_standard.v
@@ -17,15 +17,12 @@
 (**************************************************************************)
 
 
-(* Add LoadPath "." as SMTCoq.versions.standard.Int63. *)
 Require Import Bvector.
 Require Export BigNumPrelude.
-(* Require Import Int63Lib. *)
-Require Import Int31.
+Require Import Int31 Cyclic31.
 Require Export Int63Native.
-(* Require Export SMTCoq.versions.standard.Int63.Int63Native. *)
 Require Export Int63Op.
-(* Require Export SMTCoq.versions.standard.Int63.Int63Op. *)
+Require Import Psatz.
 
 Definition wB := (2^(Z_of_nat size)).
 
@@ -45,14 +42,70 @@ Local Open Scope Z_scope.
 
 (* Bijection : int63 <-> Bvector size *)
 
-Axiom to_Z_inj : forall x y, [|x|] = [|y|] -> x = y.
+Lemma to_Z_inj : forall x y, [|x|] = [|y|] -> x = y.
+Proof Ring31.Int31_canonic.
 
-Axiom of_to_Z : forall x, of_Z ([|x|]) = x.
+Lemma of_to_Z : forall x, of_Z ([|x|]) = x.
+Proof. exact phi_inv_phi. Qed.
+
+(* Comparisons *)
+Axiom eqb_refl : forall x, (x == x)%int = true.
+
+Axiom ltb_spec : forall x y, (x < y)%int = true <-> [|x|] < [|y|].
+
+Axiom leb_spec : forall x y, (x <= y)%int = true <-> [|x|] <= [|y|].
 
 (** Specification of logical operations *)
-Axiom lsl_spec : forall x p, [| x << p |] = [|x|] * 2^[|p|] mod wB.
+Lemma lsl_spec_alt p :
+  forall x, [| addmuldiv31_alt p x 0 |] = ([|x|] * 2^(Z.of_nat p)) mod wB.
+Proof.
+  induction p as [ |p IHp]; simpl; intro x.
+  - rewrite Z.mul_1_r. symmetry. apply Zmod_small. apply phi_bounded.
+  - rewrite IHp, phi_twice, Zmult_mod_idemp_l, Z.double_spec,
+            Z.mul_comm, Z.mul_assoc, Z.mul_comm,
+            Z.pow_pos_fold, Zpos_P_of_succ_nat, <- Z.add_1_r, Z.pow_add_r.
+    * reflexivity.
+    * apply Zle_0_nat.
+    * exact Z.le_0_1.
+Qed.
 
-Axiom lsr_spec : forall x p, [|x >> p|] = [|x|] / 2 ^ [|p|].
+Lemma lsl_spec x p : [| x << p |] = ([|x|] * 2^[|p|]) mod wB.
+Proof.
+  unfold lsl.
+  rewrite addmuldiv31_equiv, lsl_spec_alt, Nat2Z.inj_abs_nat, Z.abs_eq.
+  - reflexivity.
+  - now destruct (phi_bounded p).
+Qed.
+
+Lemma div_greater (p x:int) (H:Z.of_nat Int31.size <= [|p|]) : [|x|] / 2 ^ [|p|] = 0.
+Proof.
+  apply Z.div_small. destruct (phi_bounded x) as [H1 H2]. split; auto.
+  apply (Z.lt_le_trans _ _ _ H2). apply Z.pow_le_mono_r; auto.
+  exact Z.lt_0_2.
+Qed.
+
+Lemma lsr_spec x p : [|x >> p|] = [|x|] / 2 ^ [|p|].
+Proof.
+  unfold lsr. case_eq (p < 31%int31)%int; intro Heq.
+  - assert (H : [|31%int31 - p|] = 31 - [|p|]).
+    * rewrite spec_sub. rewrite Zmod_small; auto.
+      split.
+      + rewrite ltb_spec in Heq. assert (forall x y, x < y -> 0 <= y - x) by (intros;lia); auto.
+      + assert (H:forall x y z, 0 <= y /\ x < z -> x - y < z) by (intros;lia).
+        apply H. destruct (phi_bounded p). destruct (phi_bounded (31%int31)). split; auto.
+    * rewrite spec_add_mul_div.
+      + rewrite Z.add_0_l. change (phi (31%int31 - p)) with [|31%int31 - p|]. rewrite H. replace (31 - (31 - [|p|])) with [|p|] by ring. apply Zmod_small. split.
+        ++ apply div_le_0. now destruct (phi_bounded x).
+        ++ apply div_lt. apply phi_bounded.
+      + change (phi (31%int31 - p)) with [|31%int31 - p|]. rewrite H. assert (forall x y, 0 <= y -> x - y <= x) by (intros;lia). apply H0. now destruct (phi_bounded p).
+  - rewrite div_greater; auto.
+    destruct (Z.le_gt_cases [|31%int31|] [|p|]); auto.
+    rewrite <- ltb_spec in H. rewrite H in Heq. discriminate.
+Qed.
+
+
+
+
 
 Axiom land_spec: forall x y i , bit (x land y) i = bit x i && bit y i.
 
@@ -78,13 +131,6 @@ Axiom mulc_spec : forall x y, [|x|] * [|y|] = [|fst (mulc x y)|] * wB + [|snd (m
 Axiom div_spec : forall x y, [|x / y|] = [|x|] / [|y|].
 
 Axiom mod_spec : forall x y, [|x \% y|] = [|x|] mod [|y|].
-
-(* Comparisons *)
-Axiom eqb_refl : forall x, (x == x)%int = true.
-
-Axiom ltb_spec : forall x y, (x < y)%int = true <-> [|x|] < [|y|].
-
-Axiom leb_spec : forall x y, (x <= y)%int = true <-> [|x|] <= [|y|].
 
 (** Iterators *)
 
@@ -140,3 +186,10 @@ Axiom diveucl_21_spec :  forall a1 a2 b,
 
 Axiom addmuldiv_def_spec : forall p x y,
   addmuldiv p x y = addmuldiv_def p x y.
+
+
+(* 
+   Local Variables:
+   coq-load-path: ((rec "../../.." "SMTCoq"))
+   End: 
+*)
